\documentclass{article}

\usepackage{amsmath}

%usepackage{graphicx}


\begin{document}
	
	full range can either go from [0,5] or from [-1,1]
	
	\section{Algebra}
	\begin{align}
		&\text{current:   }y = x^{\frac{h_{mean}}{1-h_{mean}}}\\
		&x-h\\
		&x\\
		&x/h\\
		&xx-xh\\
	\end{align}
	
	\section{Wave mechanics and rotation}
	\begin{align}
		h(x)+h(-x)
	\end{align}
	
	
	
	\section{Calc of Variations, least time principle}
	\begin{align}
		&\frac{d}{dx}\frac{\partial}{\partial y'}\left(\frac{\sqrt{1+y'^2}}{v(x,y)}\right) = \frac{\partial}{\partial y} \left(\frac{\sqrt{1+y'^2}}{v(x,y)}\right)\\
		&v(x,y) = \frac{c}{ay+b}\\
		&\frac{d}{dx}\left(\frac{ay+b}{c}\frac{\partial}{\partial y'}\left(\sqrt{1+y'^2}\right)\right) = \sqrt{1+y'^2}\frac{\partial}{\partial y} \left(\frac{ay+b}{c}\right)\\
		&\frac{d}{dx}\left((ay+b)\frac{\partial}{\partial y'}\left(\sqrt{1+y'^2}\right)\right) = \sqrt{1+y'^2}\frac{\partial}{\partial y} \left(ay+b\right)\\
		&\frac{d}{dx}\left((ay+b)\frac{\partial}{\partial y'}\left(\sqrt{1+y'^2}\right)\right) = a\sqrt{1+y'^2}\\
		&\frac{d}{dx}\left((ay+b)\left(y'\left(1+y'^2\right)^{-\frac{1}{2}}\right)\right) = a\sqrt{1+y'^2}\\
		&\frac{d}{dx}\left((ay+b)\left(y'\right)\left(1+y'^2\right)^{-\frac{1}{2}}\right) = a\sqrt{1+y'^2}\\
		&\left(ay'\left(y'\right)\left(1+y'^2\right)^{-\frac{1}{2}}\right) + \left((ay+b)\left(y''\right)\left(1+y'^2\right)^{-\frac{1}{2}}\right) + \\
		&\left((ay+b)\left(y'\right)\left(1+y'^2\right)^{-\frac{3}{2}}\times -\frac{1}{2} \times 2y'\right) = a\sqrt{1+y'^2} \notag \\
		&\frac{ay'^2}{\sqrt{1+y'^2}} + \frac{(ay+b)\left(y''\right)}{\sqrt{\left(1+y'^2\right)}} - \frac{(ay+b)\left(y'^2\right)}{\sqrt{\left(1+y'^2\right)^3}} = a\sqrt{1+y'^2}\\
		&ay'^2 + (ay+b)\left(y''\right) - \frac{(ay+b)\left(y'^2\right)}{\left(1+y'^2\right)} = a\left(1+y'^2\right)\\
		&ayy'' - \frac{ayy'^2}{\left(1+y'^2\right)} = a\left(1+y'^2\right) - ay'^2 - by'' + \frac{by'^2}{\left(1+y'^2\right)}\\
		&y\left(ay'' - \frac{ay'^2}{\left(1+y'^2\right)}\right) = a\left(1+y'^2\right) - ay'^2 - by'' + \frac{by'^2}{\left(1+y'^2\right)}\\
		&y = \frac{a - by'' + \frac{by'^2}{\left(1+y'^2\right)}}{\left(ay'' - \frac{ay'^2}{\left(1+y'^2\right)}\right)}\\
		&b=0 \rightarrow y = \frac{a}{\left(ay'' - \frac{ay'^2}{\left(1+y'^2\right)}\right)}\\
		& u = y' \rightarrow y = \frac{1}{\left(u' - \frac{u^2}{\left(1+u^2\right)}\right)}\\
		& y = \frac{1+u^2}{\left(u'\left(1+u^2\right) - u^2\right)}\\
	\end{align}
	
	\section{simple Snells}
		\begin{align}
			&n_1\sin(\theta_1) = n_2\sin(\theta_2) \rightarrow \theta_2 = \arcsin(\frac{n_1}{n_2}\sin\theta_1)\\
			&(x_1,y_1) \text{ and } (x_2, y_2)\\
			&y=mx+b \rightarrow y-y_1 = m_1(x-x_1) \text{  and  } y-y_2 = m_2(x-x_2)\\
			& m = \tan(\theta)=\tan()\\
			&y-y_1 = \tan\theta_1(x-x_1) \text{  and  } y-y_2 = \tan\theta_2(x-x_2)\\
			&x_{interface} \text{ defined by } \tan\theta_1(x_{interface}-x_1) + y_1 = \tan\theta_2(x_{interface}-x_2) + y_2\\
			& \tan\theta_1(x_{interface}-x_1) - \tan\theta_2(x_{interface}-x_2) = y_2-y_1\\
			& \tan\theta_1x_{interface}-\tan\theta_1x_1 - \tan\theta_2x_{interface}+\tan\theta_2x_2 = y_2-y_1\\
			& \tan\theta_1x_{interface} - \tan\theta_2x_{interface} = y_2-y_1 + \tan\theta_1x_1 - \tan\theta_2x_2\\
			& x_{interface} = \frac{y_2-y_1 + \tan\theta_1x_1 - \tan\theta_2x_2}{\tan\theta_1 - \tan\theta_2}\\
			&\\
			&y-y_1 = \tan\theta_1(x-x_1) \text{  and  } y-y_2 = \tan\theta_2(x-x_2)\\
		\end{align}
	
	\section{snell bizarre idea}
	\begin{align}
		&n\sin\theta = s_0 \text{   all n's are relative}\\
		&n\sin\theta = s \text{   s as variable?}\\
			\end{align}
	
	\section{Iterated snell's law}
	\begin{align}
		&n_1\sin(\theta_1) = n_2\sin(\theta_2) =  ... = n_i\sin(\theta_i)\\
		&\theta_i = \arcsin(\frac{n_j}{n_i}\sin(\theta_j)) \forall j\\
		&\text{option 1:}\hspace{1cm} \theta_{start} = 90^o - \theta_{end}\\
		& sin(\theta) = dx/dy \ \& \ \theta = \theta(y) \ \text{related to the density}\\
		&\left. n_1\frac{d x}{d y}\right|_{y_1} = \left. n_2\frac{d x}{d y}\right|_{y_2} =  ... = \left. n_i\frac{d x}{d y}\right|_{y_i}\\
	\end{align}
	

	
	
	\section{Parametric}
	\begin{align}
		&x(t) = 
		&y(t) = 
	\end{align}
	
	
\end{document}